$$
\begin{cases} U(x_1​, x_2​)=(\alpha x_1^{\beta}​ +(1−\alpha)x_2^{\beta}​)^{1/\beta} \longrightarrow \max _{x_1, x_2} \\
I=x_1P_1 + x_2P_2 \\
1>\alpha>0
\end{cases}
$$
$$U'_{x_1} = \frac{(\alpha \beta x_1^{\beta - 1} - \frac{(1 - \alpha) \beta P_1 (\frac{I - P_1x_1}{P_2})^{\beta - 1}}{P_2}) (\alpha x_1^{\beta} + (1 - \alpha) (\frac{I - P_1x_1}{P_2})^\beta)^{\beta^{-1}-1}}{\beta}=0$$
$$
\Biggl[ \begin{array} {} \alpha \beta x_1^{\beta - 1} - P_2^{-1}(1 - \alpha) \beta P_1 (\frac{I - P_1x_1}{P_2})^{\beta - 1} =0\\
\alpha x_1^{\beta} + (1 - \alpha) (\frac{I - P_1x_1}{P_2})^\beta=0
\end{array}
$$
$$
\alpha \beta x_1^{\beta - 1}P_2 = (1 - \alpha) \beta P_1 x_2^{\beta - 1}
$$
$$
\frac{x_1}{x_2} = (\frac{(1 - \alpha)P_1}{\alpha P_2}) ^{\frac{1}{\beta - 1}}
$$